Proved fundamental lemma with annotated system

mechanization/theories/Core/Soundness/Extension/SystemAnnotated.v
@@ -19,11 +19,18 @@ Generalizable All Variables.
 (* | there_a : `({{ #n : A > s ∈ Γ : sts }} -> {{ #(S n) : A[Wk] > s ∈ Γ, B : (sb :: sts) }}) *)
 (* where "'#' x : A > s ∈ Γ : sts" := (ctx_lookup_ann x A s Γ sts) (in custom judg) : type_scope. *)
 
-Inductive wf_exp_ann {P} : ctx P -> typ P -> P -> exp P -> Prop :=
+Inductive wf_ctx_ann {P} : ctx P -> Prop :=
+| wfa_ctx_empty : {{ ⊫ ⋅ }}
+| wfa_ctx_enxtend :
+  `( {{ ⊫ Γ }} ->
+     {{ Γ ⊫ A : Sort@s > s' }} ->
+     {{ ⊫ Γ, A:Sort@s }} )
+where "⊫ Γ" := (wf_ctx_ann Γ) (in custom judg) : type_scope
+with wf_exp_ann {P} : ctx P -> typ P -> P -> exp P -> Prop :=
 (** Sorts *)
 | wfa_st :
   `( Ax P s1 s2 -> Ax P s2 s3 ->
-     {{ ⊢ Γ }} ->
+     {{ ⊫ Γ }} ->
      {{ Γ ⊫ Sort@s1 : Sort@s2 > s3 }} )
 
 (** Functions *)
@@ -49,19 +56,19 @@ Inductive wf_exp_ann {P} : ctx P -> typ P -> P -> exp P -> Prop :=
 
 (** Variables *)
 | wfa_vlookup :
-  `( {{ ⊢ Γ }} ->
+  `( {{ ⊫ Γ }} ->
      (** This premise is redundant, but helpful for soundness *)
      {{ #x : A : Sort@s ∈ Γ }} ->
      {{ Γ ⊫ #x : A > s }} )
 
 (** explicit substitutions *)
 | wfa_exp_sub_typ :
-  `( {{ Γ ⊢s σ : Δ }} ->
+  `( {{ Γ ⊫s σ : Δ }} ->
      {{ Δ ⊫ M : A > s }} ->
      {{ Δ ⊫ A : Sort@s > s' }} ->
      {{ Γ ⊫ M[σ] : A[σ] > s }} )
 | wfa_exp_sub_sort :
-  `( {{ Γ ⊢s σ : Δ }} ->
+  `( {{ Γ ⊫s σ : Δ }} ->
      {{ Δ ⊫ A : Sort@s > s' }} ->
      {{ Γ ⊫ A[σ] : Sort@s > s' }} )
 
@@ -80,152 +87,138 @@ where "Γ ⊫ M : A > s" := (wf_exp_ann Γ A s M) (in custom judg) : type_scope
 with wf_typ_ann {P} : ctx P -> typ P -> P -> Prop :=
 | wfa_typ_st :
   `( Ax P s s' ->
-     {{ ⊢ Γ }} ->
+     {{ ⊫ Γ }} ->
      {{ Γ ⊫ Sort@s > s' }} )
 | wfa_typ_exp :
   `( {{ Γ ⊫ A : Sort@s > s' }} ->
      {{ Γ ⊫ A > s }} )
-where "Γ ⊫ A > s" := (wf_typ_ann Γ A s) (in custom judg) : type_scope.
+where "Γ ⊫ A > s" := (wf_typ_ann Γ A s) (in custom judg) : type_scope
+with wf_sub_ann {P} : ctx P -> ctx P -> sub P -> Prop :=
+| wfa_sub_id :
+  `( {{ ⊫ Γ }} ->
+     {{ Γ ⊫s Id : Γ }} )
+| wfa_sub_weaken :
+  `( {{ ⊫ Γ, A:Sort@s }} ->
+     {{ Γ, A:Sort@s ⊫s Wk : Γ }} )
+| wfa_sub_compose :
+  `( {{ Γ1 ⊫s σ2 : Γ2 }} ->
+     {{ Γ2 ⊫s σ1 : Γ3 }} ->
+     {{ Γ1 ⊫s σ1∘σ2 : Γ3 }} )
+| wfa_sub_extend :
+  `( {{ Γ ⊫s σ : Δ }} ->
+     {{ Δ ⊫ A : Sort@s > s' }} ->
+     {{ Γ ⊫ M : A[σ] > s }} ->
+     {{ Γ ⊫s σ,,M : Δ, A:Sort@s }} )
+| wfa_sub_conv :
+  `( {{ Γ ⊫s σ : Δ }} ->
+     {{ ⊫ Δ' }} ->
+     {{ ⊢ Δ ≈ Δ' }} ->
+     {{ Γ ⊫s σ : Δ' }} )
+where "Γ ⊫s σ : Δ" := (wf_sub_ann Γ Δ σ) (in custom judg) : type_scope.
 
 #[export]
-Hint Constructors wf_exp_ann wf_typ_ann : mcpts.
+Hint Constructors wf_ctx_ann wf_exp_ann wf_typ_ann wf_sub_ann : mcpts.
 
-Scheme wf_exp_ann_mut_ind := Induction for wf_exp_ann Sort Prop
-with wf_typ_ann_mut_ind := Induction for wf_typ_ann Sort Prop.
-Combined Scheme syntacticwf_ann_mut_ind from
+
+Scheme wf_ctx_ann_mut_ind := Induction for wf_ctx_ann Sort Prop
+with  wf_exp_ann_mut_ind := Induction for wf_exp_ann Sort Prop
+with wf_typ_ann_mut_ind := Induction for wf_typ_ann Sort Prop
+with wf_sub_ann_mut_ind := Induction for wf_sub_ann Sort Prop.
+Combined Scheme syntactic_wf_ann_mut_ind from
+  wf_ctx_ann_mut_ind,
   wf_exp_ann_mut_ind,
-  wf_typ_ann_mut_ind.
- 
-(* Inductive wf_ctx_ann {P} : ctx P -> list P -> Prop := *)
-(* | wfa_ctx_empty : {{ ⊫ ⋅ > nil }} *)
-(* | wfa_ctx_extend : *)
-(*   `( {{ ⊫ Γ > sts }} -> *)
-(*      {{ Γ : sts ⊫ A : Sort@s > s' }} -> *)
-(*      {{ ⊫ Γ, A > (s :: sts) }} ) *)
-(* where "⊫ Γ > sts" := (wf_ctx_ann Γ sts) (in custom judg) : type_scope *)
-
-(* with wf_exp_ann {P} : ctx P -> list P -> exp P -> P -> exp P -> Prop := *)
-(* | wfa_st : *)
-(*   `( Ax P s1 s2 -> Ax P s2 s3 -> *)
-(*      {{ ⊫ Γ > sts }} -> *)
-(*      {{ Γ : sts ⊫ Sort@s1 : Sort@s2 > s3 }} ) *)
-(* (** Functions *) *)
-(* | wfa_pi : *)
-(*   `( forall (r : Ru P s1 s2 s3), *)
-(*         Ax P s3 s3' -> *)
-(*         {{ Γ : sts ⊫ A : Sort@s1 > s1' }} -> *)
-(*         {{ Γ, A : (s1 :: sts) ⊫ B : Sort@s2 > s2' }} -> *)
-(*         {{ Γ : sts ⊫ Π r A B : Sort@s3 > s3' }} ) *)
-(* | wfa_fn : *)
-(*   `( forall (r : Ru P s1 s2 s3), *)
-(*         {{ Γ : sts ⊫ A : Sort@s1 > s1' }} -> *)
-(*         {{ Γ, A : (s1 :: sts) ⊫ B : Sort@s2 > s2' }} -> *)
-(*         {{ Γ, A : (s1 :: sts) ⊫ M : B > s2 }} -> *)
-(*         {{ Γ : sts ⊫ λ r A M : Π r A B > s3 }} ) *)
-(* | wfa_app : *)
-(*   `( forall (r : Ru P s1 s2 s3), *)
-(*         {{ Γ : sts ⊫ A : Sort@s1 > s1' }} -> *)
-(*         {{ Γ, A : (s1 :: sts) ⊫ B : Sort@s2 > s2' }} -> *)
-(*         {{ Γ : sts ⊫ M : Π r A B > s3 }} -> *)
-(*         {{ Γ : sts ⊫ N : A > s1 }} -> *)
-(*         {{ Γ : sts ⊫ M N : B[Id,,N] > s2 }} ) *)
-   
-(* | wfa_vlookup : *)
-(*   `( {{ ⊫ Γ > sts }} -> *)
-(*      {{ #x : A ∈ Γ }} -> *)
-(*      {{ Γ : sts ⊫ A : Sort@s > s' }} -> *)
-(*      {{ Γ : sts ⊫ #x : A > s }} ) *)
-   
-(* (** Naturals *) *)
-(* | wfa_nat : *)
-(*   `( forall (r : Ru_nat P sn), *)
-(*         Ax P sn sn' -> *)
-(*         {{ ⊫ Γ > sts }} -> *)
-(*         {{ Γ : sts ⊫ ℕ : Sort@sn > sn' }} ) *)
-(* | wfa_zero : *)
-(*   `( forall (r : Ru_nat P sn), *)
-(*         {{ ⊫ Γ > sts }} -> *)
-(*         {{ Γ : sts ⊫ zero : ℕ > sn }} ) *)
-(* | wfa_succ : *)
-(*   `( forall (r : Ru_nat P sn), *)
-(*         {{ Γ : sts ⊫ M : ℕ > sn' }} -> *)
-(*         {{ Γ : sts ⊫ succ M : ℕ > sn }} ) *)
-(* | wfa_rec : *)
-(*   `( forall (r : Ru_nat P sn), *)
-(*         {{ Γ, ℕ : (sn :: sts) ⊫ A : Sort@sa > sa' }} -> *)
-(*         {{ Γ : sts ⊫ MZ : A[Id,,zero] > sa }} -> *)
-(*         {{ Γ, ℕ, A : (sa :: (sn :: sts)) ⊫ MS : A[Wk∘Wk,,succ #1] > sa }} -> *)
-(*         {{ Γ : sts ⊫ M : ℕ > sn }} -> *)
-(*         {{ Γ : sts ⊫ rec M return A | zero -> MZ | succ -> MS end : A[Id,,M] > sa }} ) *)
-
-(* | wfa_exp_sub : *)
-(*   `( {{ Γ : sts ⊫s σ : Δ > sts' }} -> *)
-(*      {{ Δ : sts' ⊫ M : A > s }} -> *)
-(*      {{ Γ : sts ⊫ M[σ] : A[σ] > s }} ) *)
-
-(* | wfa_exp_conv : *)
-(*   `( {{ Γ : sts ⊫ M : A > s }} -> *)
-(*      {{ Γ ⊢ A ≈ A' }} -> *)
-(*      {{ Γ : sts ⊫ M : A' > s }} ) *)
-(* | wfa_exp_conv_st : *)
-(*   `( {{ Γ : sts ⊫ M : A > s }} -> *)
-(*      {{ Γ : sts ⊫ A > s' }} -> *)
-(*      {{ Γ : sts ⊫ M : A > s' }} ) *)
-(* where "Γ : sts ⊫ M : A > s" := (wf_exp_ann Γ sts A s M) (in custom judg) : type_scope *)
-
-(* with wf_typ_ann {P} : ctx P -> list P -> typ P -> P -> Prop := *)
-(* | wfa_typ_st : *)
-(*   `( Ax P s s' -> *)
-(*      {{ ⊫ Γ > sts }} -> *)
-(*      {{ Γ : sts ⊫ Sort@s > s' }} ) *)
-(* | wfa_typ_exp : *)
-(*   `( {{ Γ : sts ⊫ A : Sort@s > s' }} -> *)
-(*      {{ Γ : sts ⊫ A > s }} ) *)
-(* | wfa_typ_clo : *)
-(*   `( {{ Γ : sts ⊫s σ : Δ > sts' }} -> *)
-(*      {{ Δ : sts' ⊫ A > s }} -> *)
-(*      {{ Γ : sts ⊫ A[σ] > s }} ) *)
-(* where "Γ : sts ⊫ A > s" := (wf_typ_ann Γ sts A s) (in custom judg) : type_scope *)
-                                                                             
-(* with wf_sub_ann {P} : ctx P -> list P -> ctx P -> list P -> sub P -> Prop := *)
-(* | wfa_sub_id : *)
-(*   `( {{ ⊫ Γ > sts }} -> *)
-(*      {{ Γ : sts ⊫s Id : Γ > sts }} ) *)
-(* | wfa_sub_weaken : *)
-(*   `( {{ ⊫ Γ, A > s :: sts }} -> *)
-(*      {{ Γ, A : s :: sts ⊫s Wk : Γ > sts }} ) *)
-(* | wfa_sub_compose : *)
-(*   `( {{ Γ1 : sts1 ⊫s σ2 : Γ2 > sts2 }} -> *)
-(*      {{ Γ2 : sts2 ⊫s σ1 : Γ3 > sts3 }} -> *)
-(*      {{ Γ1 : sts1 ⊫s σ1∘σ2 : Γ3 > sts3 }} ) *)
-(* | wfa_sub_extend : *)
-(*   `( {{ Γ : stsΓ ⊫s σ : Δ > stsΔ }} -> *)
-(*      {{ Δ : stsΔ ⊫ A : Sort@s > s' }} -> *)
-(*      {{ Γ : stsΓ ⊫ M : A[σ] > s }} -> *)
-(*      {{ Γ : stsΓ ⊫s σ,,M : Δ, A > s :: stsΔ }} ) *)
-(* | wfa_sub_conv : *)
-(*   `( {{ Γ : stsΓ ⊫s σ : Δ > stsΔ }} -> *)
-(*      {{ ⊫ Δ' > stsΔ' }} -> *)
-(*      {{ ⊢ Δ ≈ Δ' }} -> *)
-(*      {{ Γ : stsΓ ⊫s σ : Δ' > stsΔ' }} ) *)
-(* | wfa_sub_conv_sts : *)
-(*   `( {{ Γ : stsΓ ⊫s σ : Δ > stsΔ }} -> *)
-(*      {{ ⊫ Δ > stsΔ' }} -> *)
-(*      {{ Γ : stsΓ ⊫s σ : Δ > stsΔ' }} ) *)
-(* where "Γ : stsΓ ⊫s σ : Δ > stsΔ" := (wf_sub_ann Γ stsΓ Δ stsΔ σ) (in custom judg) : type_scope. *)
-
-(* #[export] *)
-(* Hint Constructors wf_ctx_ann wf_exp_ann wf_typ_ann wf_sub_ann : mcpts. *)
+  wf_typ_ann_mut_ind,
+  wf_sub_ann_mut_ind.
 
 
+#[local]
+Ltac gen_annotated_judg_IH P full_P ann_ctx ann_exp ann_sub H :=
+  match type of H with
+  | {{ ⊢ ^?Γ }} =>
+      let HΓ := fresh "HΓ" in
+      pose proof ann_ctx P full_P Γ H as HΓ
+  | {{ ^?Γ ⊢ ^?M : ^?A }} =>
+      let HM := fresh "HM" in
+      pose proof ann_exp P full_P Γ M A H as HM
+  (* | {{ ^?Γ ⊢ ^?A }} => *)
+  (*     let HA := fresh "HA" in *)
+  (*     pose proof ann_typ P full_P Γ A H as HA *)
+  | {{ ^?Γ ⊢s ^?σ : ^?Δ }} =>
+      let Hσ := fresh "Hσ" in
+      pose proof ann_sub P full_P Γ σ Δ H as Hσ
+  end.
 
-(* Scheme wf_ctx_ann_mut_ind := Induction for wf_ctx_ann Sort Prop *)
-(* with wf_exp_ann_mut_ind := Induction for wf_exp_ann Sort Prop *)
-(* with wf_sub_ann_mut_ind := Induction for wf_sub_ann Sort Prop.                                           *)
-(* Combined Scheme syntactic_wf_ann_mut_ind from *)
-(*   wf_ctx_ann_mut_ind, *)
-(*   wf_exp_ann_mut_ind, *)
-(*   wf_sub_ann_mut_ind. *)
+#[local]
+Ltac apply_fullness_once P full_P H :=
+  match type of H with
+  | Ax P ?s1 ?s2 =>
+      let s2' := fresh "s2'" in
+      assert (exists s2', Ax P s2 s2') as [s2'] by (eapply full_P)
+  | Ru P ?s1 ?s2 ?s3 =>
+      let s3' := fresh "s3'" in
+      assert (exists s3', Ax P s3 s3') as [s3'] by (eapply full_P)
+  | _ => idtac
+  end.
+
+#[local]
+Ltac apply_fullness_all P full_P :=
+  on_all_hyp: (fun H => apply_fullness_once P full_P H).
+
+Lemma wf_ctx_implies_wf_ctx_ann {P} (full_P : FullSig P) : forall {Γ : ctx P},
+    {{ ⊢ Γ }} -> {{ ⊫ Γ }}
+
+with wf_exp_implies_wf_exp_ann {P} (full_P : FullSig P) : forall {Γ : ctx P} {M A},
+    {{ Γ ⊢ M : A }} -> exists s, {{ Γ ⊫ M : A > s }}
+               
+with wf_sub_implies_wf_sub_ann {P} (full_P : FullSig P) : forall {Γ : ctx P} {σ Δ},
+    {{ Γ ⊢s σ : Δ }} -> {{ Γ ⊫s σ : Δ }}.
+Proof.
+  all: inversion_clear 1;
+    (on_all_hyp: gen_annotated_judg_IH P full_P wf_ctx_implies_wf_ctx_ann wf_exp_implies_wf_exp_ann wf_sub_implies_wf_sub_ann);
+    clear wf_ctx_implies_wf_ctx_ann wf_exp_implies_wf_exp_ann wf_sub_implies_wf_sub_ann;
+    destruct_conjs;
+    apply_fullness_all P full_P;
+    mauto 3.
+
+  - eexists; econstructor; mauto 3.
+  - assert {{ Γ ⊫ Π r A0 B : Sort@s3 > s3' }} by mauto 3.
+    assert {{ Γ ⊫ Π r A0 B > s3 }} by mauto 3.
+    assert {{ Γ ⊫ M0 : Π r A0 B > s3 }} by mauto 2.
+    assert {{ Γ ⊫ A0 > s1 }} by mauto 2.
+    assert {{ Γ ⊫ N : A0 > s1 }} by mauto 2.
+    exists s2. mauto 3.
+  - assert {{ Δ ⊫ A0 > s }} by mauto 2.
+    assert {{ Δ ⊫ M0 : A0 > s }} by mauto 2.
+    eexists; econstructor; mauto 3.
+  - admit.
+  - econstructor; mauto 3.
+    assert {{ Γ ⊫ A[σ0] : Sort@s > HM0 }} by mauto 3.
+    assert {{ Γ ⊫ A[σ0] > s }} by mauto 2.
+    mauto 3.
+Admitted.
+  
+
+Lemma wf_typ_full_implies_wf_exp {P} (full_P : FullSig P) : forall {Γ : ctx P} {A},
+    {{ Γ ⊢ A }} ->
+    exists s, {{ Γ ⊢ A : Sort@s }}.
+Proof.
+  inversion_clear 1; mauto 2.
+  assert (exists s', Ax P s s') as [s'] by (eapply full_P).
+  eexists; mauto 2.
+Qed.
+
+
+Lemma wf_typ_implies_wf_typ_ann {P} (full_P : FullSig P) : forall {Γ : ctx P} {A},
+    {{ Γ ⊢ A }} -> exists s, {{ Γ ⊫ A > s }}.
+Proof.
+  intros.
+  assert (exists s, {{ Γ ⊢ A : Sort@s }}) as [s] by (eapply wf_typ_full_implies_wf_exp; mauto 2).
+  eapply (wf_exp_implies_wf_exp_ann full_P) in H0.
+  destruct_conjs.
+  mauto 3.
+Qed.
+
+
 
 
 (* #[local] *)
@@ -548,22 +541,27 @@ Combined Scheme syntacticwf_ann_mut_ind from
 (*     do 2 eexists; mauto 2. *)
 (* Qed. *)
 
-(* Lemma wf_judg_ann_implies_wf_judg {P} : *)
-(*   (forall (Γ : ctx P) sts, {{ ⊫ Γ > sts }} -> {{ ⊢ Γ }}) /\ *)
-(*     (forall (Γ : ctx P) sts A s M, {{ Γ : sts ⊫ M : A > s }} -> {{ Γ ⊢ M : A }}) /\ *)
-(*     (forall (Γ : ctx P) sts Δ sts' σ, {{ Γ : sts ⊫s σ : Δ > sts' }} -> {{ Γ ⊢s σ : Δ }}). *)
-(* Proof. *)
-(*   eapply syntactic_wf_ann_mut_ind; mauto 2. *)
-(* Qed. *)
+Lemma wf_judg_ann_implies_wf_judg {P} :
+  (forall (Γ : ctx P), {{ ⊫ Γ }} -> {{ ⊢ Γ }}) /\
+    (forall (Γ : ctx P) A s M, {{ Γ ⊫ M : A > s }} -> {{ Γ ⊢ M : A }}) /\
+    (forall (Γ : ctx P) A s, {{ Γ ⊫ A > s }} -> {{ Γ ⊢ A }}) /\    
+    (forall (Γ : ctx P) Δ σ, {{ Γ ⊫s σ : Δ }} -> {{ Γ ⊢s σ : Δ }}).
+Proof.
+  eapply syntactic_wf_ann_mut_ind; mauto 2.
+Qed.
 
-(* Corollary wf_ctx_ann_implies_wf_ctx {P} : forall {Γ : ctx P} {sts}, *)
-(*     {{ ⊫ Γ > sts }} -> {{ ⊢ Γ }}. *)
-(* Proof. intros; eapply wf_judg_ann_implies_wf_judg; mauto 2. Qed. *)
+Corollary wf_ctx_ann_implies_wf_ctx {P} : forall {Γ : ctx P},
+    {{ ⊫ Γ }} -> {{ ⊢ Γ }}.
+Proof. intros; eapply wf_judg_ann_implies_wf_judg; mauto 2. Qed.
 
-(* Corollary wf_exp_ann_implies_wf_exp {P} : forall {Γ : ctx P} {sts A s M}, *)
-(*     {{ Γ : sts ⊫ M : A > s }} -> {{ Γ ⊢ M : A }}. *)
-(* Proof. intros; eapply wf_judg_ann_implies_wf_judg; mauto 2. Qed. *)
+Corollary wf_exp_ann_implies_wf_exp {P} : forall {Γ : ctx P} {A s M},
+    {{ Γ ⊫ M : A > s }} -> {{ Γ ⊢ M : A }}.
+Proof. intros; eapply wf_judg_ann_implies_wf_judg; mauto 2. Qed.
 
-(* Corollary wf_sub_ann_implies_wf_sub {P} : forall {Γ : ctx P} {sts Δ sts' σ}, *)
-(*     {{ Γ : sts ⊫s σ : Δ > sts' }} -> {{ Γ ⊢s σ : Δ }}. *)
-(* Proof. intros; eapply wf_judg_ann_implies_wf_judg; mauto 2. Qed. *)
+Corollary wf_typ_ann_implies_wf_typ {P} : forall {Γ : ctx P} {A s},
+    {{ Γ ⊫ A > s }} -> {{ Γ ⊢ A }}.
+Proof. intros; eapply wf_judg_ann_implies_wf_judg; mauto 2. Qed.
+
+Corollary wf_sub_ann_implies_wf_sub {P} : forall {Γ : ctx P} {Δ σ},
+    {{ Γ ⊫s σ : Δ }} -> {{ Γ ⊢s σ : Δ }}.
+Proof. intros; eapply wf_judg_ann_implies_wf_judg; mauto 2. Qed.
