mechanization/theories/Core/Soundness/FundamentalTheorem.v
@@ -11,74 +11,38 @@ From McPTS.Core.Soundness.Extension Require Import SystemAnnotated.
 Import Domain_Notations.
 
 Section soundness_fundamental.
-  #[local]
-  Ltac gen_soundness_IH P pred_P full_P soundness_ctx soundness_exp soundness_typ soundness_sub H :=
-  match type of H with
-  | {{ ⊢ ^?Γ }} =>
-      let HΓ := fresh "HΓ" in
-      pose proof soundness_ctx P pred_P full_P Γ H as HΓ
-  | {{ ^?Γ ⊫ ^?M : ^?A > ^?s }} =>
-      let HM := fresh "HM" in
-      pose proof soundness_exp P pred_P full_P Γ A s M H as HM
-  | {{ ^?Γ ⊫ ^?A > ^?s }} =>
-      let HA := fresh "HA" in
-      pose proof soundness_typ P pred_P full_P Γ A s H as HA
-  | {{ ^?Γ ⊢s ^?σ : ^?Δ }} =>
-      let Hσ := fresh "Hσ" in
-      pose proof soundness_sub P pred_P full_P Γ Δ σ H as Hσ
-  end.
-   
-  Theorem soundness_fundamental_ctx_ann {P} (pred_P : PredicativeSig P) (full_P : FullSig P) :
-    forall Γ, {{ ⊢ Γ }} -> {{ ⟪ pred_P ⟫ ⊩ Γ }}
-  with soundness_fundamental_exp_ann {P} (pred_P : PredicativeSig P) (full_P : FullSig P) :
-    forall Γ A s M, {{ Γ ⊫ M : A > s }} -> {{ ⟪ pred_P ⟫ Γ ⊩ M : A > s }}
-  with soundness_fundamental_typ_ann {P} (pred_P : PredicativeSig P) (full_P : FullSig P) :
-    forall Γ A s, {{ Γ ⊫ A > s }} -> {{ ⟪ pred_P ⟫ Γ ⊩ A > s }}
-  with soundness_fundamental_sub_ann {P} (pred_P : PredicativeSig P) (full_P : FullSig P) :
-    forall Γ Δ σ, {{ Γ ⊢s σ : Δ }} -> {{ ⟪ pred_P ⟫ Γ ⊩s σ : Δ }}.
+  Theorem soundness_fundamental {P} (pred_P : PredicativeSig P) (full_P : FullSig P) :
+    (forall Γ, {{ ⊫ Γ }} -> {{ ⟪ pred_P ⟫ ⊩ Γ }}) /\
+      (forall Γ A s M, {{ Γ ⊫ M : A > s }} -> {{ ⟪ pred_P ⟫ Γ ⊩ M : A > s }}) /\
+      (forall Γ A s, {{ Γ ⊫ A > s }} -> {{ ⟪ pred_P ⟫ Γ ⊩ A > s }}) /\
+      (forall Γ Δ σ, {{ Γ ⊫s σ : Δ }} -> {{ ⟪ pred_P ⟫ Γ ⊩s σ : Δ }}).
   Proof.
-    all: inversion_clear 1;
-      (on_all_hyp: gen_soundness_IH P pred_P full_P soundness_fundamental_ctx_ann soundness_fundamental_exp_ann soundness_fundamental_typ_ann soundness_fundamental_sub_ann);
-      clear soundness_fundamental_ctx_ann soundness_fundamental_exp_ann soundness_fundamental_typ_ann soundness_fundamental_sub_ann;
-      mauto 2.
+    eapply syntactic_wf_ann_mut_ind; mauto 3; intros.
 
-    - (* Context extensions. Need to define proper annotations {{ ⊫ Γ }} *)
-      admit.
-    - (* wf_typ_sort *)
-      assert (exists s', Ax P s s') as [s'] by (eapply full_P).
-      assert {{ ⟪ pred_P ⟫ Γ ⊩ Sort@s0 : Sort@s > s' }} by mauto 2.
-      destruct H2 as [SbΓ []].
-      econstructor; split; mauto 2.
-      intros.
-      destruct_glu_rel_exp_with_sub.
-      simplify_evals.
-      invert_glu_sort_elem H7.
-      unfold sort_glu_exp_pred' in *.
-      unfold glu_sort_typ_rec in *.
-      eapply H6 in H8.
-      destruct_conjs.      
-      econstructor; mauto 2.      
-      
-    - (* wf_typ_exp *)
-      destruct HM as [SbΓ []].
-      eexists; split; mauto 2.
-      intros.
-      destruct_glu_rel_exp_with_sub.
-      simplify_evals.
-      invert_glu_sort_elem H5.
-      unfold sort_glu_exp_pred' in *.
-      unfold glu_sort_typ_rec in *.
-      eapply H5 in H6.
-      destruct_conjs.      
-      econstructor; mauto 2.
-    - (* Substitution extensions (need to properly define annotated judgments {{ Γ ⊫s σ : Δ }} *)
-      admit.
-    - (* Conversion for substitutions (need another lemma) *)
-      admit.
-      
-  Admitted.
+    eapply glu_rel_exp_conv; mauto 3.
+  Qed.
+
+  #[local]
+  Ltac solve_it pred_P full_P := pose proof soundness_fundamental pred_P full_P; firstorder.
   
+  Corollary soundness_fundamental_ctx_ann {P} (pred_P : PredicativeSig P) (full_P : FullSig P) :
+    forall Γ, {{ ⊫ Γ }} -> {{ ⟪ pred_P ⟫ ⊩ Γ }}.
+  Proof. solve_it pred_P full_P. Qed.
+  
+  Corollary soundness_fundamental_exp_ann {P} (pred_P : PredicativeSig P) (full_P : FullSig P) :
+    forall Γ A s M, {{ Γ ⊫ M : A > s }} -> {{ ⟪ pred_P ⟫ Γ ⊩ M : A > s }}.
+  Proof. solve_it pred_P full_P. Qed.
+  
+  Corollary soundness_fundamental_typ_ann {P} (pred_P : PredicativeSig P) (full_P : FullSig P) :
+    forall Γ A s, {{ Γ ⊫ A > s }} -> {{ ⟪ pred_P ⟫ Γ ⊩ A > s }}.
+  Proof. solve_it pred_P full_P. Qed.
+  
+  Corollary soundness_fundamental_sub_ann {P} (pred_P : PredicativeSig P) (full_P : FullSig P) :
+    forall Γ Δ σ, {{ Γ ⊫s σ : Δ }} -> {{ ⟪ pred_P ⟫ Γ ⊩s σ : Δ }}.
+  Proof. solve_it pred_P full_P. Qed.  
 
+
+  
   Theorem soundness_fundamental_ctx {P} (pred_P : PredicativeSig P) (full_P : FullSig P) :
     forall Γ, {{ ⊢ Γ }} -> exists sts, {{ ⟪ pred_P ⟫ ⊩ Γ : sts }}.
   Proof.
