mechanization/theories/Core/Soundness/TermStructureCases.v
@@ -215,4 +215,3 @@ Qed.
 
 #[export]
 Hint Resolve glu_rel_exp_conv_sort : mcpts.
-                                         
